\documentclass{article}
\usepackage{epsfig}
\usepackage{amsmath}
\pagestyle{empty}
\begin{document}
$d = \sqrt{(x_2 - x_1)^2 + (y_2 - y_1)^2 + (z_2 - z_1)^2}$
\pagebreak

$ \frac{P_r}{P_t} = \frac{A_r A_t}{d^2\lambda^2} $
\pagebreak

$ A_{isotr.} = \frac{\lambda^2}{4\pi} $
\pagebreak

$ \frac{P_r}{P_t} = \frac{\lambda^2}{(4 \pi d)^2} $
\pagebreak

$ P_r = \frac{P_t G_t G_r \lambda^2}{(4 \pi d)^2 L}$
\pagebreak

$ RX_{dB} = TX_{dB} + 10\mathrm{log_{10}} \frac{\lambda^2}{(4 \pi d)^2 L}$
\pagebreak

$ P_r $
\pagebreak

$ P_t $
\pagebreak

$ G_t $
\pagebreak

$ G_r $
\pagebreak

$ \lambda $
\pagebreak

$ d $
\pagebreak

$ L $
\pagebreak

$ d = \frac{kD^2}{8\lambda} $
\pagebreak

$ d = \frac{1}{8}\lambda $
\pagebreak

$ a_[i]^{m_[i] - 2} \mathrm{mod m_[i]} $
\pagebreak

\end{document}
